Continuations, function type, and its variance.

theories/typing/function.v
@@ -1,123 +1,88 @@
+From iris.base_logic Require Import big_op.
 From iris.proofmode Require Import tactics.
 From iris.program_logic Require Import hoare.
 From lrust.lifetime Require Import borrow.
 From lrust.typing Require Export type.
-From lrust.typing Require Import type_incl typing.
+From lrust.typing Require Import type_incl typing lft_contexts type_context cont_context.
 
 Section fn.
   Context `{typeG Σ}.
 
-  Program Definition cont {n : nat} (ρ : vec val n → @perm Σ) :=
-    {| ty_size := 1;
-       ty_own tid vl := (∃ f, ⌜vl = [f]⌝ ∗
-          ∀ vl, ρ vl tid -∗ na_own tid ⊤
-                 -∗ WP f (map of_val vl) {{λ _, False}})%I;
-       ty_shr κ tid N l := True%I |}.
-  Next Obligation.
-    iIntros (n ρ tid vl) "H". iDestruct "H" as (f) "[% _]". by subst.
-  Qed.
-  Next Obligation. intros. by iIntros "_ _". Qed.
-  Next Obligation. intros. by iIntros "_ _ _". Qed.
-
-  (* TODO : For now, functions are not Send. This means they cannot be
-     called in another thread than the one that created it.  We will
-     need Send functions when dealing with multithreading ([fork]
-     needs a Send closure). *)
-  Program Definition fn {A n} (ρ : A -> vec val n → @perm Σ) : type :=
+  Program Definition fn {A n} (E : A → elctx)
+          (tys : A → vec type n) (ty : A → type) : type :=
     {| st_size := 1;
-       st_own tid vl := (∃ f, ⌜vl = [f]⌝ ∗ ∀ x vl,
-         {{ ρ x vl tid ∗ na_own tid ⊤ }} f (map of_val vl) {{λ _, False}})%I |}.
+       st_own tid vl := (∃ f, ⌜vl = [f]⌝ ∗ □ ∀ (x : A) (args : vec val n) (k : val),
+         typed_body (E x) []
+                    [CctxElt k [] 1 (λ v, [TCtx_holds (v!!!0) (ty x)])]
+                    (zip_with (TCtx_holds ∘ of_val) args (tys x))
+                    (f (of_val <$> (args : list val))))%I |}.
   Next Obligation.
-    iIntros (x n ρ tid vl) "H". iDestruct "H" as (f) "[% _]". by subst.
+    iIntros (A n E tys ty tid vl) "H". iDestruct "H" as (f) "[% _]". by subst.
   Qed.
 
-  Lemma ty_incl_cont {n} ρ ρ1 ρ2 :
-    Duplicable ρ → (∀ vl : vec val n, ρ ∗ ρ2 vl ⇒ ρ1 vl) →
-    ty_incl ρ (cont ρ1) (cont ρ2).
+  Lemma fn_subtype_ty A n E0 E L tys1 tys2 ty1 ty2:
+    (∀ x, Forall2 (subtype (E0 ++ E x) L) (tys2 x : vec _ _) (tys1 x : vec _ _)) →
+    (∀ x, subtype (E0 ++ E x) L (ty1 x) (ty2 x)) →
+    subtype E0 L (@fn A n E tys1 ty1) (@fn A n E tys2 ty2).
   Proof.
-    iIntros (? Hρ1ρ2 tid) "#LFT #Hρ!>". iSplit; iIntros "!#*H"; last by auto.
-    iDestruct "H" as (f) "[% Hwp]". subst. iExists _. iSplit. done.
-    iIntros (vl) "Hρ2 Htl". iApply ("Hwp" with ">[-Htl] Htl").
-    iApply (Hρ1ρ2 with "LFT"). by iFrame.
+    intros Htys Hty. apply subtype_simple_type=>//=.
+    iIntros (_ ?) "#LFT #HE0 #HL0 Hf". iDestruct "Hf" as (f) "[% #Hf]". subst.
+    iExists f. iSplit. done. rewrite /typed_body. iIntros "!# * _ HE HL HC HT".
+    iDestruct (elctx_interp_persist with "HE") as "#HE'".
+    iApply ("Hf" with "* LFT HE HL [HC] [HT]").
+    - iIntros "HE". unfold cctx_interp. iIntros (e) "He".
+      iDestruct "He" as %->%elem_of_list_singleton. iIntros (ret) "HL HT".
+      iSpecialize ("HC" with "HE"). unfold cctx_elt_interp.
+      iApply ("HC" $! (CctxElt _ _ _ _) with "[%] * HL >").
+        by apply elem_of_list_singleton.
+      iApply (subtype_tctx_incl with "LFT [HE0] HL0 HT"). by apply Hty.
+      rewrite /elctx_interp_0 big_sepL_app. by iSplit.
+    - rewrite /tctx_interp
+         -(fst_zip (tys1 x) (tys2 x)) ?vec_to_list_length //
+         -{1}(snd_zip (tys1 x) (tys2 x)) ?vec_to_list_length //
+         !zip_with_fmap_r !(zip_with_zip (λ _ _, (_ ∘ _) _ _)) !big_sepL_fmap.
+      iApply big_sepL_impl. iSplit; last done. iIntros "{HT}!#".
+      iIntros (i [p [ty1' ty2']]) "#Hzip H /=".
+      iDestruct "H" as (v) "[? Hown]". iExists v. iFrame.
+      rewrite !lookup_zip_with.
+      iDestruct "Hzip" as %(? & ? & ([? ?] & (? & Hty'1 &
+        (? & Hty'2 & [=->->])%bind_Some)%bind_Some & [=->->->])%bind_Some)%bind_Some.
+      specialize (Htys x). eapply Forall2_lookup_lr in Htys; try done.
+      iApply (Htys.(subtype_own _ _ _ _) with "LFT [] HL0 Hown").
+      rewrite /elctx_interp_0 big_sepL_app. by iSplit.
   Qed.
 
-  Lemma ty_incl_fn {A n} ρ ρ1 ρ2 :
-    Duplicable ρ → (∀ (x : A) (vl : vec val n), ρ ∗ ρ2 x vl ⇒ ρ1 x vl) →
-    ty_incl ρ (fn ρ1) (fn ρ2).
-  Proof.
-    iIntros (? Hρ1ρ2 tid) "#LFT #Hρ!>". iSplit; iIntros "!#*#H".
-    - iDestruct "H" as (f) "[% Hwp]". subst. iExists _. iSplit. done.
-      iIntros (x vl) "!#[Hρ2 Htl]". iApply ("Hwp" with ">").
-      iFrame. iApply (Hρ1ρ2 with "LFT"). by iFrame.
-    - iSplit; last done. simpl. iDestruct "H" as (vl0) "[? [Hvl|H†]]".
-      + iExists vl0. iFrame "#". iLeft. iNext. iDestruct "Hvl" as (f) "[% Hwp]".
-        iExists f. iSplit. done. iIntros (x vl) "!#[Hρ2 Htl]".
-        iApply ("Hwp" with ">"). iFrame. iApply (Hρ1ρ2 with "LFT >"). by iFrame.
-      + iExists _. iFrame "#". by iRight.
-  Qed.
+  (* Lemma ty_incl_fn_specialize {A B n} (f : A → B) ρ ρfn : *)
+  (*   ty_incl ρ (fn (n:=n) ρfn) (fn (ρfn ∘ f)). *)
+  (* Proof. *)
+  (*   iIntros (tid) "_ _!>". iSplit; iIntros "!#*H". *)
+  (*   - iDestruct "H" as (fv) "[%#H]". subst. iExists _. iSplit. done. *)
+  (*     iIntros (x vl). by iApply "H". *)
+  (*   - iSplit; last done. *)
+  (*     iDestruct "H" as (fvl) "[?[Hown|H†]]". *)
+  (*     + iExists _. iFrame. iLeft. iNext. *)
+  (*       iDestruct "Hown" as (fv) "[%H]". subst. iExists _. iSplit. done. *)
+  (*       iIntros (x vl). by iApply "H". *)
+  (*     + iExists _. iFrame. by iRight. *)
+  (* Qed. *)
 
-  Lemma ty_incl_fn_cont {A n} ρ ρf (x : A) :
-    ty_incl ρ (fn ρf) (cont (n:=n) (ρf x)).
-  Proof.
-    iIntros (tid) "#LFT _!>". iSplit; iIntros "!#*H"; last by iSplit.
-    iDestruct "H" as (f) "[%#H]". subst. iExists _. iSplit. done.
-    iIntros (vl) "Hρf Htl". iApply "H". by iFrame.
-  Qed.
-
-  Lemma ty_incl_fn_specialize {A B n} (f : A → B) ρ ρfn :
-    ty_incl ρ (fn (n:=n) ρfn) (fn (ρfn ∘ f)).
-  Proof.
-    iIntros (tid) "_ _!>". iSplit; iIntros "!#*H".
-    - iDestruct "H" as (fv) "[%#H]". subst. iExists _. iSplit. done.
-      iIntros (x vl). by iApply "H".
-    - iSplit; last done.
-      iDestruct "H" as (fvl) "[?[Hown|H†]]".
-      + iExists _. iFrame. iLeft. iNext.
-        iDestruct "Hown" as (fv) "[%H]". subst. iExists _. iSplit. done.
-        iIntros (x vl). by iApply "H".
-      + iExists _. iFrame. by iRight.
-  Qed.
-
-  Lemma typed_fn {A n} `{Duplicable _ ρ, Closed (f :b: xl +b+ []) e} θ :
-    length xl = n →
-    (∀ (a : A) (vl : vec val n) (fv : val) e',
-        subst_l xl (map of_val vl) e = Some e' →
-        typed_program (fv ◁ fn θ ∗ (θ a vl) ∗ ρ) (subst' f fv e')) →
-    typed_step_ty ρ (Rec f xl e) (fn θ).
-  Proof.
-    iIntros (Hn He tid) "!#(#HEAP&#LFT&#Hρ&$)".
-    assert (Rec f xl e = RecV f xl e) as -> by done. iApply wp_value'.
-    rewrite has_type_value.
-    iLöb as "IH". iExists _. iSplit. done. iIntros (a vl) "!#[Hθ?]".
-    assert (is_Some (subst_l xl (map of_val vl) e)) as [e' He'].
-    { clear -Hn. revert xl Hn e. induction vl=>-[|x xl] //=. by eauto.
-      intros ? e. edestruct IHvl as [e' ->]. congruence. eauto. }
-    iApply wp_rec; try done.
-    { apply List.Forall_forall=>?. rewrite in_map_iff=>-[?[<- _]].
-      rewrite to_of_val. eauto. }
-    iNext. iApply He. done. iFrame "∗#". by rewrite has_type_value.
-  Qed.
-
-  Lemma typed_cont {n} `{Closed (f :b: xl +b+ []) e} ρ θ :
-    length xl = n →
-    (∀ (fv : val) (vl : vec val n) e',
-        subst_l xl (map of_val vl) e = Some e' →
-        typed_program (fv ◁ cont (λ vl, ρ ∗ θ vl)%P ∗ (θ vl) ∗ ρ) (subst' f fv e')) →
-    typed_step_ty ρ (Rec f xl e) (cont θ).
-  Proof.
-    iIntros (Hn He tid) "!#(#HEAP&#LFT&Hρ&$)". specialize (He (RecV f xl e)).
-    assert (Rec f xl e = RecV f xl e) as -> by done. iApply wp_value'.
-    rewrite has_type_value.
-    iLöb as "IH". iExists _. iSplit. done. iIntros (vl) "Hθ ?".
-    assert (is_Some (subst_l xl (map of_val vl) e)) as [e' He'].
-    { clear -Hn. revert xl Hn e. induction vl=>-[|x xl] //=. by eauto.
-      intros ? e. edestruct IHvl as [e' ->]. congruence. eauto. }
-    iApply wp_rec; try done.
-    { apply List.Forall_forall=>?. rewrite in_map_iff=>-[?[<- _]].
-      rewrite to_of_val. eauto. }
-    iNext. iApply He. done. iFrame "∗#". rewrite has_type_value.
-    iExists _. iSplit. done. iIntros (vl') "[Hρ Hθ] Htl".
-    iDestruct ("IH" with "Hρ") as (f') "[Hf' IH']".
-    iDestruct "Hf'" as %[=<-]. iApply ("IH'" with "Hθ Htl").
-  Qed.
+  (* Lemma typed_fn {A n} `{Duplicable _ ρ, Closed (f :b: xl +b+ []) e} θ : *)
+  (*   length xl = n → *)
+  (*   (∀ (a : A) (vl : vec val n) (fv : val) e', *)
+  (*       subst_l xl (map of_val vl) e = Some e' → *)
+  (*       typed_program (fv ◁ fn θ ∗ (θ a vl) ∗ ρ) (subst' f fv e')) → *)
+  (*   typed_step_ty ρ (Rec f xl e) (fn θ). *)
+  (* Proof. *)
+  (*   iIntros (Hn He tid) "!#(#HEAP&#LFT&#Hρ&$)". *)
+  (*   assert (Rec f xl e = RecV f xl e) as -> by done. iApply wp_value'. *)
+  (*   rewrite has_type_value. *)
+  (*   iLöb as "IH". iExists _. iSplit. done. iIntros (a vl) "!#[Hθ?]". *)
+  (*   assert (is_Some (subst_l xl (map of_val vl) e)) as [e' He']. *)
+  (*   { clear -Hn. revert xl Hn e. induction vl=>-[|x xl] //=. by eauto. *)
+  (*     intros ? e. edestruct IHvl as [e' ->]. congruence. eauto. } *)
+  (*   iApply wp_rec; try done. *)
+  (*   { apply List.Forall_forall=>?. rewrite in_map_iff=>-[?[<- _]]. *)
+  (*     rewrite to_of_val. eauto. } *)
+  (*   iNext. iApply He. done. iFrame "∗#". by rewrite has_type_value. *)
+  (* Qed. *)
 End fn.
