theories/typing/lft_contexts.v
@@ -9,33 +9,63 @@ Section lft_contexts.
 
   (* External lifetime contexts. *)
 
-  Inductive lectx_elt : Type :=
-  | LECtx_Alive κ
-  | LECtx_Incl κ κ'.
-  Definition lectx := list lectx_elt.
+  Inductive elctx_elt : Type :=
+  | ELCtx_Alive κ
+  | ELCtx_Incl κ κ'.
+  Definition elctx := list elctx_elt.
 
-  Definition lectx_elt_interp (x : lectx_elt) (q : Qp) : iProp Σ :=
+  Definition elctx_elt_interp (x : elctx_elt) (q : Qp) : iProp Σ :=
     match x with
-    | LECtx_Alive κ => q.[κ]
-    | LECtx_Incl κ κ' => κ ⊑ κ'
+    | ELCtx_Alive κ => q.[κ]
+    | ELCtx_Incl κ κ' => κ ⊑ κ'
     end%I.
-  Global Instance lectx_elt_interp_fractional x:
-    Fractional (lectx_elt_interp x).
-  Proof. destruct x; unfold lectx_elt_interp; apply _. Qed.
-  Typeclasses Opaque lectx_elt_interp.
+  Global Instance elctx_elt_interp_fractional x:
+    Fractional (elctx_elt_interp x).
+  Proof. destruct x; unfold elctx_elt_interp; apply _. Qed.
+  Typeclasses Opaque elctx_elt_interp.
+  Definition elctx_elt_interp_0 (x : elctx_elt) : iProp Σ :=
+    match x with
+    | ELCtx_Alive κ => True
+    | ELCtx_Incl κ κ' => κ ⊑ κ'
+    end%I.
+  Global Instance elctx_elt_interp_0_persistent x:
+    PersistentP (elctx_elt_interp_0 x).
+  Proof. destruct x; apply _. Qed.
+  Typeclasses Opaque elctx_elt_interp_0.
 
-  Definition lectx_interp (E : lectx) (q : Qp) : iProp Σ :=
-    ([∗ list] x ∈ E, lectx_elt_interp x q)%I.
-  Global Instance lectx_interp_fractional E:
-    Fractional (lectx_interp E).
+  Lemma elctx_elt_interp_persist x q :
+    elctx_elt_interp x q -∗ elctx_elt_interp_0 x.
+  Proof. destruct x; by iIntros "?/=". Qed.
+
+  Definition elctx_interp (E : elctx) (q : Qp) : iProp Σ :=
+    ([∗ list] x ∈ E, elctx_elt_interp x q)%I.
+  Global Instance elctx_interp_fractional E:
+    Fractional (elctx_interp E).
   Proof. intros ??. rewrite -big_sepL_sepL. by setoid_rewrite <-fractional. Qed.
-  Global Instance lectx_interp_as_fractional E q:
-    AsFractional (lectx_interp E q) (lectx_interp E) q.
-  Proof. done. Qed.
-  Global Instance lectx_interp_permut:
-    Proper ((≡ₚ) ==> eq ==> (⊣⊢)) lectx_interp.
+  Global Instance elctx_interp_as_fractional E q:
+    AsFractional (elctx_interp E q) (elctx_interp E) q.
+  Proof. split. done. apply _. Qed.
+  Global Instance elctx_interp_permut:
+    Proper ((≡ₚ) ==> eq ==> (⊣⊢)) elctx_interp.
   Proof. intros ????? ->. by apply big_opL_permutation. Qed.
-  Typeclasses Opaque lectx_interp.
+  Typeclasses Opaque elctx_interp.
+
+  Definition elctx_interp_0 (E : elctx) : iProp Σ :=
+    ([∗ list] x ∈ E, elctx_elt_interp_0 x)%I.
+  Global Instance elctx_interp_0_persistent E:
+    PersistentP (elctx_interp_0 E).
+  Proof. apply _. Qed.
+  Global Instance elctx_interp_0_permut:
+    Proper ((≡ₚ) ==> (⊣⊢)) elctx_interp_0.
+  Proof. intros ???. by apply big_opL_permutation. Qed.
+  Typeclasses Opaque elctx_interp_0.
+
+  Lemma elctx_interp_persist x q :
+    elctx_interp x q -∗ elctx_interp_0 x.
+  Proof.
+    unfold elctx_interp, elctx_interp_0. f_equiv. intros _ ?.
+    apply elctx_elt_interp_persist.
+  Qed.
 
   (* Local lifetime contexts. *)
 
@@ -59,6 +89,15 @@ Section lft_contexts.
   Qed.
   Typeclasses Opaque llctx_elt_interp.
 
+  Definition llctx_elt_interp_0 (x : llctx_elt) : Prop :=
+    let κ' := foldr (∪) static (x.2) in (∃ κ0, x.1 = κ' ∪ κ0).
+  Lemma llctx_elt_interp_persist x q :
+    llctx_elt_interp x q -∗ ⌜llctx_elt_interp_0 x⌝.
+  Proof.
+    iIntros "H". unfold llctx_elt_interp.
+    iDestruct "H" as (κ0) "[% _]". by iExists κ0.
+  Qed.
+
   Definition llctx_interp (L : llctx) (q : Qp) : iProp Σ :=
     ([∗ list] x ∈ L, llctx_elt_interp x q)%I.
   Global Instance llctx_interp_fractional L:
@@ -66,13 +105,22 @@ Section lft_contexts.
   Proof. intros ??. rewrite -big_sepL_sepL. by setoid_rewrite <-fractional. Qed.
   Global Instance llctx_interp_as_fractional L q:
     AsFractional (llctx_interp L q) (llctx_interp L) q.
-  Proof. done. Qed.
+  Proof. split. done. apply _. Qed.
   Global Instance llctx_interp_permut:
     Proper ((≡ₚ) ==> eq ==> (⊣⊢)) llctx_interp.
   Proof. intros ????? ->. by apply big_opL_permutation. Qed.
   Typeclasses Opaque llctx_interp.
 
-  Context (E : lectx) (L : llctx).
+  Definition llctx_interp_0 (L : llctx) : Prop :=
+    ∀ x, x ∈ L → llctx_elt_interp_0 x.
+  Lemma llctx_interp_persist L q :
+    llctx_interp L q -∗ ⌜llctx_interp_0 L⌝.
+  Proof.
+    iIntros "H". iIntros (x ?). iApply llctx_elt_interp_persist.
+    unfold llctx_interp. by iApply (big_sepL_elem_of with "H").
+  Qed.
+
+  Context (E : elctx) (L : llctx).
 
   (* Lifetime inclusion *)
 
@@ -80,40 +128,39 @@ Section lft_contexts.
      "equivalence" of lifetimes. If so, TODO : add it, and the
      corresponding [Proper] instances for the relevent types. *)
   Definition incl κ κ' : Prop :=
-    ∀ qE qL, lectx_interp E qE -∗ llctx_interp L qL -∗ κ ⊑ κ'.
+    elctx_interp_0 E -∗ ⌜llctx_interp_0 L⌝ -∗ κ ⊑ κ'.
 
   Global Instance incl_preorder : PreOrder incl.
   Proof.
     split.
-    - iIntros (???) "_ _". iApply lft_incl_refl.
-    - iIntros (??? H1 H2 ??) "HE HL". iApply (lft_incl_trans with "[#] [#]").
+    - iIntros (?) "_ _". iApply lft_incl_refl.
+    - iIntros (??? H1 H2) "#HE #HL". iApply (lft_incl_trans with "[#] [#]").
       iApply (H1 with "HE HL"). iApply (H2 with "HE HL").
   Qed.
 
   Lemma incl_static κ : incl κ static.
-  Proof. iIntros (??) "_ _". iApply lft_incl_static. Qed.
+  Proof. iIntros "_ _". iApply lft_incl_static. Qed.
 
   Lemma incl_local κ κ' κs : (κ, κs) ∈ L → κ' ∈ κs → incl κ κ'.
   Proof.
-    intros ? Hκ'κs ??. rewrite /llctx_interp /llctx_elt_interp big_sepL_elem_of //.
-    iIntros "_ H". iDestruct "H" as (κ0) "[H _]". simpl. iDestruct "H" as %->.
+    iIntros (? Hκ'κs) "_ H". iDestruct "H" as %(κ0 & EQ). done. simpl in EQ; subst.
     iApply lft_le_incl. etrans; last by apply gmultiset_union_subseteq_l.
     clear -Hκ'κs. induction Hκ'κs.
     - apply gmultiset_union_subseteq_l.
     - etrans. done. apply gmultiset_union_subseteq_r.
   Qed.
 
-  Lemma incl_external κ κ' : LECtx_Incl κ κ' ∈ E → incl κ κ'.
+  Lemma incl_external κ κ' : ELCtx_Incl κ κ' ∈ E → incl κ κ'.
   Proof.
-    intros ???. rewrite /lectx_interp /lectx_elt_interp big_sepL_elem_of //.
-      by iIntros "$ _".
+    iIntros (?) "H _".
+    rewrite /elctx_interp_0 /elctx_elt_interp_0 big_sepL_elem_of //. done.
   Qed.
 
   (* Lifetime aliveness *)
 
   Definition alive (κ : lft) : Prop :=
-    ∀ F qE qL, ⌜↑lftN ⊆ F⌝ -∗ lectx_interp E qE -∗ llctx_interp L qL ={F}=∗
-          ∃ q', q'.[κ] ∗ (q'.[κ] ={F}=∗ lectx_interp E qE ∗ llctx_interp L qL).
+    ∀ F qE qL, ⌜↑lftN ⊆ F⌝ -∗ elctx_interp E qE -∗ llctx_interp L qL ={F}=∗
+          ∃ q', q'.[κ] ∗ (q'.[κ] ={F}=∗ elctx_interp E qE ∗ llctx_interp L qL).
 
   Lemma alive_static : alive static.
   Proof.
@@ -127,7 +174,7 @@ Section lft_contexts.
     iDestruct (big_sepL_lookup_acc with "HL2") as "[Hκ Hclose]". done.
     iDestruct "Hκ" as (κ0) "(EQ & Htok & #Hend)". simpl. iDestruct "EQ" as %->.
     iAssert (∃ q', q'.[foldr union static κs] ∗
-      (q'.[foldr union static κs] ={F}=∗ lectx_interp E qE ∗ llctx_interp L (qL / 2)))%I
+      (q'.[foldr union static κs] ={F}=∗ elctx_interp E qE ∗ llctx_interp L (qL / 2)))%I
       with ">[HE HL1]" as "H".
     { move:(qL/2)%Qp=>qL'. clear HL. iClear "Hend".
       iInduction Hκs as [|κ κs Hκ ?] "IH" forall (qE qL').
@@ -147,10 +194,10 @@ Section lft_contexts.
     rewrite /llctx_interp /llctx_elt_interp. iApply "Hclose". iExists κ0. iFrame. auto.
   Qed.
 
-  Lemma alive_lectx κ: LECtx_Alive κ ∈ E → alive κ.
+  Lemma alive_elctx κ: ELCtx_Alive κ ∈ E → alive κ.
   Proof.
     iIntros ([i HE]%elem_of_list_lookup_1 F qE qL) "% HE $ !>".
-    rewrite /lectx_interp /lectx_elt_interp.
+    rewrite /elctx_interp /elctx_elt_interp.
     iDestruct (big_sepL_lookup_acc with "HE") as "[Hκ Hclose]". done.
     iExists qE. iFrame. iIntros "?!>". by iApply "Hclose".
   Qed.
@@ -158,7 +205,8 @@ Section lft_contexts.
   Lemma alive_incl κ κ': alive κ → incl κ κ' → alive κ'.
   Proof.
     iIntros (Hal Hinc F qE qL) "% HE HL".
-    iAssert (κ ⊑ κ')%I with "[#]" as "#Hincl". by iApply (Hinc with "HE HL").
+    iAssert (κ ⊑ κ')%I with "[#]" as "#Hincl". iApply (Hinc with "[HE] [HL]").
+      by iApply elctx_interp_persist. by iApply llctx_interp_persist.
     iMod (Hal with "[%] HE HL") as (q') "[Htok Hclose]". done.
     iMod (lft_incl_acc with "Hincl Htok") as (q'') "[Htok Hclose']". done.
     iExists q''. iIntros "{$Htok}!>Htok". iApply ("Hclose" with ">").
@@ -167,37 +215,38 @@ Section lft_contexts.
 
   (* External lifetime context satisfiability *)
 
-  Definition lectx_sat E' : Prop :=
-    ∀ qE qL F, ⌜↑lftN ⊆ F⌝ -∗ lectx_interp E qE -∗ llctx_interp L qL ={F}=∗
-      ∃ qE', lectx_interp E' qE' ∗
-       (lectx_interp E' qE' ={F}=∗ lectx_interp E qE ∗ llctx_interp L qL).
+  Definition elctx_sat E' : Prop :=
+    ∀ qE qL F, ⌜↑lftN ⊆ F⌝ -∗ elctx_interp E qE -∗ llctx_interp L qL ={F}=∗
+      ∃ qE', elctx_interp E' qE' ∗
+       (elctx_interp E' qE' ={F}=∗ elctx_interp E qE ∗ llctx_interp L qL).
 
-  Lemma lectx_sat_nil : lectx_sat [].
+  Lemma elctx_sat_nil : elctx_sat [].
   Proof.
-    iIntros (qE qL F) "%$$". iExists 1%Qp. rewrite /lectx_interp big_sepL_nil. auto.
+    iIntros (qE qL F) "%$$". iExists 1%Qp. rewrite /elctx_interp big_sepL_nil. auto.
   Qed.
 
-  Lemma lectx_sat_alive E' κ :
-    alive κ → lectx_sat E' → lectx_sat (LECtx_Alive κ :: E').
+  Lemma elctx_sat_alive E' κ :
+    alive κ → elctx_sat E' → elctx_sat (ELCtx_Alive κ :: E').
   Proof.
     iIntros (Hκ HE' qE qL F) "% [HE1 HE2] [HL1 HL2]".
     iMod (Hκ with "[%] HE1 HL1") as (q) "[Htok Hclose]". done.
     iMod (HE' with "[%] HE2 HL2") as (q') "[HE' Hclose']". done.
     destruct (Qp_lower_bound q q') as (q0 & q2 & q'2 & -> & ->). iExists q0.
-    rewrite {5 6}/lectx_interp big_sepL_cons /=.
+    rewrite {5 6}/elctx_interp big_sepL_cons /=.
     iDestruct "Htok" as "[$ Htok]". iDestruct "HE'" as "[Hf HE']".
-    iSplitL "Hf". by rewrite /lectx_interp.
+    iSplitL "Hf". by rewrite /elctx_interp.
     iIntros "!>[Htok' ?]". iMod ("Hclose" with "[$Htok $Htok']") as "[$$]".
-    iApply "Hclose'". iFrame. by rewrite /lectx_interp.
+    iApply "Hclose'". iFrame. by rewrite /elctx_interp.
   Qed.
 
-  Lemma lectx_sat_incl E' κ κ' :
-    incl κ κ' → lectx_sat E' → lectx_sat (LECtx_Incl κ κ' :: E').
+  Lemma elctx_sat_incl E' κ κ' :
+    incl κ κ' → elctx_sat E' → elctx_sat (ELCtx_Incl κ κ' :: E').
   Proof.
     iIntros (Hκκ' HE' qE qL F) "% HE HL".
-    iAssert (κ ⊑ κ')%I with "[#]" as "#Hincl". by iApply (Hκκ' with "HE HL").
+    iAssert (κ ⊑ κ')%I with "[#]" as "#Hincl". iApply (Hκκ' with "[HE] [HL]").
+      by iApply elctx_interp_persist. by iApply llctx_interp_persist.
     iMod (HE' with "[%] HE HL") as (q) "[HE' Hclose']". done.
-    iExists q. rewrite {1 2 4 5}/lectx_interp big_sepL_cons /=.
+    iExists q. rewrite {1 2 4 5}/elctx_interp big_sepL_cons /=.
     iIntros "{$Hincl $HE'}!>[_ ?]". by iApply "Hclose'".
   Qed.
 End lft_contexts.
